@base  <http://rdf.naturallexicon.org/prototypes/ont#>.
@prefix : <#>
@prefix owl: <http://www.w3.org/2002/07/owl#>.
@prefix rdf: <http://www.w3.org/1999/02/22-rdf-syntax-ns#>.
@prefix rdfs: <http://www.w3.org/2000/01/rdf-schema#>.


<#> rdfs:comment """ 
Defines a lightweight knowledge representation scheme that supports definitions of prototypes, which can appear in elaboration chains, whose properties aggregate according to an aggregation policy.
""";
.

<#PrototypeClass> rdfs:subClassof rdf:Property;
    rdfs:comment """
        Refers to a class pertinent to prototypes.
        """;
    .

<#Prototype> a :PrototypeClass;
  rdfs:comment """
  Refers to objects which can be described by elaboration properties.
  """;
.

<#PrototypeProperty> rdfs:subClassof rdf:Property;
    rdfs:comment """
        Refers to a property that affects the description of a prototype's referent.
        """;
    .

<#elaborates> a :ProtypeProperty;
    a :TransclusiveProperty;
  rdfs:comment """
  <subordinate> proto:elaborates <superordinate>.
  
  Asserts that <superordinate> acquires properties from <superordinate>,
  subject to the proto:ElaborationPolicy of said properties.
        """;
    rdfs:domain :Prototype;
    rdfs:range :Prototype;
    owl:seeAlso :ElaborationPolicy;
    .

<#Elaboration> a :PrototypeProperty;
  rdfs:comment """
  <prototype> elaboration <value>
  Asserts that <value> is a property of <prototype>, subject to the rules of 
  elaboration.
  """;
.

<#ElaborationPolicy> a :PrototypeClass;
  rdfs:comment """
  Refers to one of proto:Exclusive, proto:Inclusive, proto:Occlusive,
   proto:Transclusive
  
  Exclusive meaning that it is an error for elaborating prototypes to make new assertions 
  for this property.

  Inclusive meaning that assertions made by elaborating prototypes will be
  conjoined with other such assertions.

  Occlusive meaning that assertions made by elaborating prototypes override
  assertions made by superior nodes in the prototype lineage.

  Transclusive meaning that assertions made by elaborating prototypes do not
    attach to the referent, but rather inform the inference of the referent.
    
  """
.

<#ExclusiveAggregation> rdfs:subClassOf :ElaborationPolicy;
  rdfs:comment """
  Refers to an aggregation policy wherein it is an error for elaborating 
  prototypes to make new assertions for properties in this class.
  Examples would be unique identifiers and things like biological species.
  """
.

<#InclusiveAggregation> rdfs:subClassOf :ElaborationPolicy;
  rdfs:comment """
  Refers to an aggregation policy wherein assertions made by elaborating 
  prototypes will be conjoined with other such assertions within the 
  elaboration lineage. This is the default.
  """;
.

<#OcclusiveAggregation> rdfs:subClassOf :ElaborationPolicy;
  rdfs:comment """
  Refers to an aggregation policy wherein assertions made by elaborating 
  prototypes override assertions made by superior nodes in the elaboration
  lineage.
  """;
.

<#TransclusiveAggregation> rdfs:subClassOf :ElaborationPolicy;
    rdfs:comment """
        Refers to a policy wherein the property in question does not attach ot the resulting referent, but rather characterizes some aspect of the inference process. An example would be the proto:elaborates.
        """;
    .
    
<#hasAggregationPolicy>
  rdfs:domain :ElaborationProperty;
  rdfs:range :AggregationPolicy;
  rdfs:comment """
        This ensemble:
  <property> proto:hasAggregationPolicy <policy>.
  <parent> <property> <value>.
  <child> <elaborates> <parent>.
  
  Asserts that <policy> applies when inferring <value> for <child>.

  """;
.

<#ExclusiveProperty> rdfs:subClassOf :ElaborationProperty;
    owl:subClassOf
    [a owl:Restriction;
     owl:onProperty :hasAggregationPolicy;
     owl:hasValue :ExclusiveAggregation;
    ];
    .

<#InclusiveProperty> rdfs:subClassOf :ElaborationProperty;
    owl:subClassOf
    [a owl:Restriction;
     owl:onProperty :hasAggregationPolicy;
     owl:hasValue :InclusiveAggregation;
    ];
    .

<#OcclusiveProperty> rdfs:subClassOf :ElaborationProperty;
    owl:subClassOf
    [a owl:Restriction;
     owl:onProperty :hasAggregationPolicy;
     owl:hasValue :OcclusiveAggregation;
    ];
    .

<#TransclusiveProperty> rdfs:subClassOf :ElaborationProperty;
    owl:subClassOf
    [a owl:Restriction;
     owl:onProperty :hasAggregationPolicy;
     owl:hasValue :TransclusiveAggregation;
    ];
    .

<#hasParameter> a :TransclusiveProperty;
   rdfs:comment """
        <prototype> proto:hasParameter <property>

Asserts that <prototype> should specify at least one value for
<property> to be well-formed.

        """;
    .
    
    